Adding functions

Core.v
@@ -1,12 +1,10 @@
-From Coq Require Import Init.Nat.
 From Coq Require Import List.
 
-From Elo Require Export Array.
-From Elo Require Export Map.
-
-Import ListNotations.
-
-Definition name := String.string.
+From Elo Require Import Util.
+From Elo Require Import Array.
+From Elo Require Import Map.
+ 
+Definition id := Strings.String.string.
 Definition num := nat.
 
 (* Notations *)
@@ -15,108 +13,103 @@ Reserved Notation "'[' id ':=' x ']' t"
   (at level 20, id constr).
 Reserved Notation "t '--[' eff ']-->' t'"
   (at level 40).
-Reserved Notation "m / ths '==[' ceff ']==>' m' / ths'"
-  (at level 40, ths at next level, ceff at next level, m' at next level).
+Reserved Notation "m / t '==[' eff ']==>' m' / t'"
+  (at level 40, t at next level, eff at next level, m' at next level).
+Reserved Notation "m / ths '~~[' tid , eff ']~~>' m' / ths'"
+  (at level 40, ths at next level, tid at next level, eff at next level,
+                m' at next level).
 Reserved Notation "mt / Gamma '|--' t 'is' T"
   (at level 40, Gamma at next level).
 
 (* Types *)
 
 Inductive typ : Set :=
-  | TY_Void
+  | TY_Unit
   | TY_Num
   | TY_Ref : typ -> typ
   | TY_Fun : typ -> typ -> typ
   .
 
+Theorem typ_eq_dec : forall (t1 t2 : typ),
+  {t1 = t2} + {t1 <> t2}.
+Proof.
+  intros. decide equality; eauto.
+Qed.
+
 (* Terms *)
 
 Inductive tm : Set :=
-  | TM_Nil
-  | TM_Num : num -> tm
-  | TM_Id : name -> tm
-  | TM_Fun : name -> typ -> tm -> typ -> tm
-  | TM_Loc : num -> tm
-  | TM_Load : tm -> tm
-  | TM_New : tm -> tm
-  | TM_Asg : tm -> tm -> tm
-  | TM_Call : tm -> tm -> tm
-  | TM_Seq : tm -> tm -> tm
-  | TM_Let : name -> typ -> tm -> tm -> tm
+  | TM_Unit
+  | TM_Num   : num -> tm
+  | TM_Loc   : num -> tm
+  | TM_New   : tm  -> tm
+  | TM_Load  : tm  -> tm
+  | TM_Asg   : tm  -> tm  -> tm
+  | TM_Id    : id  -> tm
+  | TM_Fun   : id  -> typ -> tm -> tm
+  | TM_Call  : tm  -> tm  -> tm
+  | TM_Seq   : tm  -> tm  -> tm
+  | TM_Spawn : tm  -> tm
   .
+
+Theorem tm_eq_dec : forall (t1 t2 : tm),
+  {t1 = t2} + {t1 <> t2}.
+Proof.
+  intros. decide equality; 
+  eauto using PeanoNat.Nat.eq_dec, Strings.String.string_dec, typ_eq_dec.
+Qed.
 
 (* Values *)
 
 Inductive value : tm -> Prop :=
-  | V_Nil : value TM_Nil
+  | V_Nil : value TM_Unit
   | V_Num : forall n, value (TM_Num n)
   | V_Loc : forall i, value (TM_Loc i)
-  | V_Fun : forall p P block R, value (TM_Fun p P block R)
+  | V_Fun : forall x X t, value (TM_Fun x X t)
   .
 
 (* Effects *)
 
+Definition addr := nat.
+
 Inductive effect : Set :=
   | EF_None
-  | EF_Alloc (ad : num) (t : tm)
-  | EF_Load  (ad : num) (t : tm)
-  | EF_Store (ad : num) (t : tm)
+  | EF_Alloc (ad : addr) (t : tm)
+  | EF_Load  (ad : addr) (t : tm)
+  | EF_Store (ad : addr) (t : tm)
+  | EF_Spawn (t : tm)
   .
 
-Inductive ceffect : Set :=
-  | CEF_None  (tid : nat)
-  | CEF_Alloc (tid : nat) (ad : nat) (t : tm)
-  | CEF_Load  (tid : nat) (ad : nat) (t : tm)
-  | CEF_Store (tid : nat) (ad : nat) (t : tm)
-  .
+Theorem effect_eq_dec : forall (e1 e2 : effect),
+  {e1 = e2} + {e1 <> e2}.
+Proof.
+  intros. decide equality; eauto using PeanoNat.Nat.eq_dec, tm_eq_dec.
+Qed.
 
-(* Auxiliary Aliases *)
-
-Definition ctx := map typ.
-Definition mem := list tm.
-Definition threads := list tm.
-Definition memtyp := list typ.
-Definition get_typ := get TY_Void.
-Definition get_tm  := get TM_Nil.
-Definition get_ctx := get (@empty typ).
-
-(* Operational Semantics *)
+(* Substitution *)
 
 Local Infix "=?" := String.eqb (at level 70, no associativity).
 
-Fixpoint subst (id : name) (x t : tm) : tm :=
+Fixpoint subst (id : id) (x t : tm) : tm :=
   match t with
-  | TM_Nil => t
-  | TM_Num _ => t
-  | TM_Id id' =>
-      if id =? id' then x else t
-  | TM_Fun p P block R =>
-      if id =? p then t else TM_Fun p P ([id := x] block) R
-  | TM_New t' =>
-      [id := x] t'
-  | TM_Loc _ => t
-  | TM_Load t' =>
-      TM_Load ([id := x] t')
-  | TM_Asg t' e =>
-      TM_Asg ([id := x] t') ([id := x] e)
-  | TM_Call f a =>
-      TM_Call ([id := x] f) ([id := x] a)
-  | TM_Seq t1 t2 =>
-      TM_Seq ([id := x] t1) ([id := x] t2)
-  | TM_Let id' E e t' =>
-      TM_Let id' E ([id := x] e) (if id =? id' then t' else [id := x] t')
+  | TM_Unit         => t
+  | TM_Num _        => t
+  | TM_Loc _        => t
+  | TM_New t'       => TM_New  ([id := x] t')
+  | TM_Load t'      => TM_Load ([id := x] t')
+  | TM_Asg t1 t2    => TM_Asg  ([id := x] t1) ([id := x] t2)
+  | TM_Id id'       => if id =? id' then x else t
+  | TM_Fun id' X t' => if id =? id' then t else TM_Fun id' X ([id := x] t')
+  | TM_Call t1 t2   => TM_Call ([id := x] t1) ([id := x] t2)
+  | TM_Seq t1 t2    => TM_Seq  ([id := x] t1) ([id := x] t2)
+  (* | TM_Spawn t'     => TM_Spawn ([id := x] t') *)
+  | TM_Spawn _      => t
   end
   where "'[' id ':=' x ']' t" := (subst id x t).
 
+(* Operational Semantics *)
+
 Inductive step : tm -> effect -> tm -> Prop :=
-  (* Load *)
-  | ST_Load1 : forall t t' eff,
-    t --[eff]--> t' ->
-    TM_Load t --[eff]--> TM_Load t'
-
-  | ST_Load : forall ad t,
-    TM_Load (TM_Loc ad) --[EF_Load ad t]--> t
-
   (* New *)
   | ST_New1 : forall t t' eff,
     t --[eff]--> t' ->
@@ -125,6 +118,14 @@ Inductive step : tm -> effect -> tm -> Prop :=
   | ST_New : forall t ad,
     value t ->
     TM_New t --[EF_Alloc ad t]--> TM_Loc ad
+
+  (* Load *)
+  | ST_Load1 : forall t t' eff,
+    t --[eff]--> t' ->
+    TM_Load t --[eff]--> TM_Load t'
+
+  | ST_Load : forall ad t,
+    TM_Load (TM_Loc ad) --[EF_Load ad t]--> t
 
   (* Asg *)
   | ST_Asg1 : forall l l' r eff,
@@ -138,115 +139,149 @@ Inductive step : tm -> effect -> tm -> Prop :=
 
   | ST_Asg : forall t ad,
     value t ->
-    TM_Asg (TM_Loc ad) t --[EF_Store ad t]--> TM_Nil
+    TM_Asg (TM_Loc ad) t --[EF_Store ad t]--> TM_Unit
 
   (* Call *)
-  | ST_Call1 : forall f f' a eff,
+  | ST_Call1 : forall f f' x eff,
     f --[eff]--> f' ->
-    TM_Call f a --[eff]--> TM_Call f' a
+    TM_Call f x --[eff]--> TM_Call f' x
 
-  | ST_Call2 : forall f a a' eff,
+  | ST_Call2 : forall f x x' eff,
     value f ->
-    a --[eff]--> a' ->
-    TM_Call f a --[eff]--> TM_Call f a'
+    x --[eff]--> x' ->
+    TM_Call f x --[eff]--> TM_Call f x'
 
-  | ST_Call : forall p P block R a,
-    value a ->
-    TM_Call (TM_Fun p P block R) a --[EF_None]--> [p := a] block
+  | ST_Call : forall id X t x,
+    value x ->
+    TM_Call (TM_Fun id X t) x --[EF_None]--> [id := x] t
 
   (* Seq *)
-  | ST_Seq1 : forall t1 t2 t eff,
-    t1 --[eff]--> t2 ->
-    TM_Seq t1 t --[eff]--> TM_Seq t2 t
+  | ST_Seq1 : forall t1 t1' t2 eff,
+    t1 --[eff]--> t1' ->
+    TM_Seq t1 t2 --[eff]--> TM_Seq t1' t2
 
-  | ST_Seq : forall t,
-    TM_Seq TM_Nil t --[EF_None]--> t
+  | ST_Seq : forall t v,
+    value v ->
+    TM_Seq v t --[EF_None]--> t
 
-  (* Let *)
-  | ST_Let1 : forall id E e e' t eff,
-    e --[eff]--> e' ->
-    TM_Let id E e t --[eff]--> TM_Let id E e' t
-
-  | ST_Let : forall id E e t,
-    value e ->
-    TM_Let id E e t --[EF_None]--> [id := e] t
+  (* Spawn *)
+  | ST_Spawn : forall t,
+    TM_Spawn t --[EF_Spawn t]--> TM_Unit
 
   where "t '--[' eff ']-->' t'" := (step t eff t').
 
+Ltac induction_step :=
+  match goal with
+    | H : _ --[?e]--> _ |- _ => remember e as eff; induction H
+  end.
+
+(* Memory Step *)
+
+Definition mem := list tm.
+Definition getTM := get TM_Unit.
+
+Inductive mstep : mem -> tm -> effect -> mem -> tm -> Prop :=
+  | MST_None : forall m t t',
+    t --[EF_None]--> t' ->
+    m / t ==[EF_None]==> m / t'
+
+  | MST_Alloc : forall m t t' ad v,
+    ad = length m ->
+    t --[EF_Alloc ad v]--> t' ->
+    m / t ==[EF_Alloc ad v]==> (add m v) / t'
+
+  | MST_Load : forall m t t' ad,
+    t --[EF_Load ad (getTM m ad)]--> t' ->
+    m / t ==[EF_Load ad (getTM m ad) ]==> m / t'
+
+  | MST_Store : forall m t t' ad v,
+    ad < length m ->
+    t --[EF_Store ad v]--> t' ->
+    m / t ==[EF_Store ad v]==> (set m ad v) / t'
+
+  where "m / t '==[' eff ']==>' m' / t'" := (mstep m t eff m' t').
+
+Ltac inversion_mstep' :=
+  match goal with
+    | H : _ / _ ==[_]==> _ / _ |- _ => inversion H; subst
+  end.
+
+Ltac inversion_mstep :=
+  match goal with
+    | H : _ / _ ==[_]==> _ / _ |- _ => inversion H; subst; clear H
+  end.
+
 (* Concurrent Step *)
 
-Inductive cstep : mem -> threads -> mem -> threads -> ceffect -> Prop :=
-  | CST_None : forall tid m ths t,
-    tid < length ths ->
-    (get_tm ths tid) --[EF_None]--> t ->
-    m / ths ==[ CEF_None tid ]==> m / (set ths tid t)
+Definition threads := list tm.
 
-  | CST_Alloc : forall tid m ths v t,
-    tid < length ths ->
-    (get_tm ths tid) --[EF_Alloc (length m) v]--> t ->
-    m / ths ==[ CEF_Alloc tid (length m) v ]==> (add m v) / (set ths tid t)
+Inductive cstep : mem -> threads -> nat -> effect -> mem -> threads -> Prop :=
+  | CST_Mem : forall m m' t' ths tid eff block,
+      tid < length ths ->
+      eff <> EF_Spawn block ->
+      m / (getTM ths tid) ==[eff]==> m' / t' ->
+      m / ths ~~[tid, eff]~~> m' / (set ths tid t')
 
-  | CST_Load : forall tid m ths ad t,
-    tid < length ths ->
-    (get_tm ths tid) --[EF_Load ad (get_tm m ad)]--> t ->
-    m / ths ==[ CEF_Load tid ad (get_tm m ad) ]==> m / (set ths tid t)
+  | CST_Spawn : forall m t' ths tid block,
+      tid < length ths ->
+      (getTM ths tid) --[EF_Spawn block]--> t' ->
+      m / ths ~~[tid, EF_Spawn block]~~> m / (add (set ths tid t') block)
 
-  | CST_Store : forall tid m ths ad v t,
-    tid < length ths ->
-    ad < length m ->
-    (get_tm ths tid) --[EF_Store ad v]--> t ->
-    m / ths ==[ CEF_Store tid ad v ]==> (set m ad v) / (set ths tid t)
+  where "m / ths '~~[' tid ,  eff ']~~>' m' / ths'" :=
+    (cstep m ths tid eff m' ths').
 
-  where "m / ths '==[' ceff ']==>' m' / ths'" := (cstep m ths m' ths' ceff).
+Ltac inversion_cstep :=
+  match goal with
+    | H : _ / _ ~~[_, _]~~> _ / _ |- _ => inversion H; subst; clear H
+  end.
 
 (* Typing *)
 
+Definition memtyp := list typ.
+Definition ctx := map typ.
+Definition getTY := get TY_Unit.
+
 Inductive well_typed_term (mt : memtyp) : ctx -> tm -> typ -> Prop :=
   | T_Nil : forall Gamma,
-    mt / Gamma |-- TM_Nil is TY_Void
+    mt / Gamma |-- TM_Unit is TY_Unit
 
   | T_Num : forall Gamma n,
     mt / Gamma |-- (TM_Num n) is TY_Num
 
-  | T_Id : forall Gamma id T,
-    lookup Gamma id = Some T ->
-    mt / Gamma |-- (TM_Id id) is T
-
-  | T_Fun : forall Gamma p P block R,
-    mt / (update Gamma p P) |-- block is R ->
-    mt / Gamma |-- (TM_Fun p P block R) is (TY_Fun P R)
-
   | T_Loc : forall Gamma ad,
     ad < length mt ->
-    mt / Gamma |-- (TM_Loc ad) is TY_Ref (get_typ mt ad)
-
-  | T_Load : forall Gamma t T,
-    mt / Gamma |-- t is TY_Ref T ->
-    mt / Gamma |-- (TM_Load t) is T
+    mt / Gamma |-- (TM_Loc ad) is TY_Ref (get TY_Unit mt ad )
 
   | T_New : forall Gamma t T,
     mt / Gamma |-- t is T ->
     mt / Gamma |-- (TM_New t) is (TY_Ref T)
 
-  | T_Asg : forall Gamma t e T,
-    mt / Gamma |-- t is (TY_Ref T) ->
-    mt / Gamma |-- e is T ->
-    mt / Gamma |-- (TM_Asg t e) is TY_Void
+  | T_Load : forall Gamma t T,
+    mt / Gamma |-- t is TY_Ref T ->
+    mt / Gamma |-- (TM_Load t) is T
 
-  | T_Call : forall Gamma f a P R,
-    mt / Gamma |-- f is (TY_Fun P R) ->
-    mt / Gamma |-- a is P ->
-    mt / Gamma |-- (TM_Call f a) is R
+  | T_Asg : forall Gamma t1 t2 T,
+    mt / Gamma |-- t1 is (TY_Ref T) ->
+    mt / Gamma |-- t2 is T ->
+    mt / Gamma |-- (TM_Asg t1 t2) is TY_Unit
 
-  | T_Seq : forall Gamma t t' T,
-    mt / Gamma |-- t  is TY_Void ->
-    mt / Gamma |-- t' is T ->
-    mt / Gamma |-- (TM_Seq t t') is T
+  | T_Fun : forall Gamma x t X T,
+    mt / (update Gamma x X) |-- t is T ->
+    mt / Gamma |-- (TM_Fun x X t) is (TY_Fun X T)
 
-  | T_Let : forall Gamma id e t E T,
-    mt / Gamma |-- e is E ->
-    mt / (update Gamma id E) |-- t is T ->
-    mt / Gamma |-- (TM_Let id E e t) is T
+  | T_Call : forall Gamma f x X T,
+    mt / Gamma |-- f is (TY_Fun X T) ->
+    mt / Gamma |-- x is X ->
+    mt / Gamma |-- (TM_Call f x) is T
+
+  | T_Seq : forall Gamma t1 t2 T1 T2,
+    mt / Gamma |-- t1 is T1 ->
+    mt / Gamma |-- t2 is T2 ->
+    mt / Gamma |-- (TM_Seq t1 t2) is T2
+
+  | T_Spawn : forall Gamma t T,
+    mt / empty |-- t is T ->
+    mt / Gamma |-- (TM_Spawn t) is TY_Unit
 
   where "mt / Gamma '|--' t 'is' T" := (well_typed_term mt Gamma t T).
 
