Access.v
@@ -1,7 +1,8 @@
 From Coq Require Logic.ClassicalFacts.
 
+From Elo Require Import Util.
 From Elo Require Import Array.
-From Elo Require Import Core0.
+From Elo Require Import Core.
 
 Inductive access (m : mem) : tm -> addr -> Prop :=
   | access_mem : forall ad ad',
@@ -27,6 +28,18 @@ Inductive access (m : mem) : tm -> addr -> Prop :=
     access m r ad ->
     access m (TM_Asg l r) ad
 
+  | access_fun : forall x X t ad,
+    access m t ad ->
+    access m (TM_Fun x X t) ad
+
+  | access_call1 : forall t1 t2 ad,
+    access m t1 ad ->
+    access m (TM_Call t1 t2) ad
+
+  | access_call2 : forall t1 t2 ad,
+    access m t2 ad ->
+    access m (TM_Call t1 t2) ad
+
   | access_seq1 : forall t1 t2 ad,
     access m t1 ad ->
     access m (TM_Seq t1 t2) ad
@@ -49,60 +62,113 @@ Local Axiom excluded_middle : ClassicalFacts.excluded_middle.
 
 Lemma access_dec : forall m t ad,
   (access m t ad) \/ (~ access m t ad).
-Proof.
-  eauto using excluded_middle.
-Qed.
+Proof. eauto using excluded_middle. Qed.
 
 Ltac inversion_access :=
   match goal with
-    | H : access _ TM_Nil       _ |- _ => inversion H; clear H
-    | H : access _ (TM_Num _)   _ |- _ => inversion H; clear H
-    | H : access _ (TM_Loc _)   _ |- _ => inversion H; subst; clear H
-    | H : access _ (TM_New _)   _ |- _ => inversion H; subst; clear H
-    | H : access _ (TM_Load _)  _ |- _ => inversion H; subst; clear H
-    | H : access _ (TM_Asg _ _) _ |- _ => inversion H; subst; clear H
-    | H : access _ (TM_Seq _ _) _ |- _ => inversion H; subst; clear H
-    | H : access _ (TM_Spawn _) _ |- _ => inversion H; clear H
+  | H : access _ TM_Unit        _ |- _ => inversion H; clear H
+  | H : access _ (TM_Num _)     _ |- _ => inversion H; clear H
+  | H : access _ (TM_Loc _)     _ |- _ => inversion H; subst; clear H
+  | H : access _ (TM_New _)     _ |- _ => inversion H; subst; clear H
+  | H : access _ (TM_Load _)    _ |- _ => inversion H; subst; clear H
+  | H : access _ (TM_Asg _ _)   _ |- _ => inversion H; subst; clear H
+  | H : access _ (TM_Id _)      _ |- _ => inversion H; clear H
+  | H : access _ (TM_Fun _ _ _) _ |- _ => inversion H; subst; clear H
+  | H : access _ (TM_Call _ _)  _ |- _ => inversion H; subst; clear H
+  | H : access _ (TM_Seq _ _)   _ |- _ => inversion H; subst; clear H
+  | H : access _ (TM_Spawn _)   _ |- _ => inversion H; clear H
   end.
 
-Lemma inversion_not_access_loc : forall m ad ad',
+(* -------------------------------------------------------------------------- *)
+(* not_access --------------------------------------------------------------- *)
+(* -------------------------------------------------------------------------- *)
+
+Local Ltac solve_not_access :=
+  intros; intros ?; inversion_access; eauto.
+
+Lemma not_access_new : forall m t ad,
+  ~ access m t ad ->
+  ~ access m (TM_New t) ad.
+Proof. solve_not_access. Qed.
+
+Lemma not_access_load : forall m t ad,
+  ~ access m t ad ->
+  ~ access m (TM_Load t) ad.
+Proof. solve_not_access. Qed.
+
+Lemma not_access_fun : forall m x X t ad,
+  ~ access m t ad ->
+  ~ access m (TM_Fun x X t) ad.
+Proof. solve_not_access. Qed.
+
+Lemma not_access_call : forall m t1 t2 ad,
+  ~ access m t1 ad ->
+  ~ access m t2 ad ->
+  ~ access m (TM_Call t1 t2) ad.
+Proof. solve_not_access. Qed.
+
+Lemma not_access_asg : forall m t1 t2 ad,
+  ~ access m t1 ad ->
+  ~ access m t2 ad ->
+  ~ access m (TM_Asg t1 t2) ad.
+Proof. solve_not_access. Qed.
+
+Lemma not_access_seq : forall m t1 t2 ad,
+  ~ access m t1 ad ->
+  ~ access m t2 ad ->
+  ~ access m (TM_Seq t1 t2) ad.
+Proof. solve_not_access. Qed.
+
+(* -------------------------------------------------------------------------- *)
+(* inversion_not_access ----------------------------------------------------- *)
+(* -------------------------------------------------------------------------- *)
+
+Local Ltac solve_inversion_not_access :=
+  intros;
+  match goal with
+  | |- _ /\ _ => split 
+  | |- _  => idtac
+  end;
+  intros F; inversion F; subst; eauto using access.
+
+Local Lemma inversion_not_access_loc : forall m ad ad',
   ~ access m (TM_Loc ad) ad' ->
   ~ access m (getTM m ad) ad'.
-Proof.
-  intros * ? F. inversion F; subst; eauto using access.
-Qed.
+Proof. solve_inversion_not_access. Qed.
 
-Lemma inversion_not_access_new : forall m t ad,
+Local Lemma inversion_not_access_new : forall m t ad,
   ~ access m (TM_New t) ad ->
   ~ access m t ad.
-Proof.
-  intros * ? F. inversion F; subst; eauto using access.
-Qed.
+Proof. solve_inversion_not_access. Qed.
 
-Lemma inversion_not_access_load : forall m t ad,
+Local Lemma inversion_not_access_load : forall m t ad,
   ~ access m (TM_Load t) ad ->
   ~ access m t ad.
-Proof.
-  intros * ? F. inversion F; subst; eauto using access.
-Qed.
+Proof. solve_inversion_not_access. Qed.
 
-Lemma inversion_not_access_asg : forall m l r ad,
+Local Lemma inversion_not_access_asg : forall m l r ad,
   ~ access m (TM_Asg l r) ad ->
   ~ access m l ad /\ ~ access m r ad.
-Proof.
-  intros * ?. split; intros F; inversion F; subst; eauto using access.
-Qed.
+Proof. solve_inversion_not_access. Qed.
 
-Lemma inversion_not_access_seq : forall m t1 t2 ad,
+Local Lemma inversion_not_access_fun : forall m x X t ad,
+  ~ access m (TM_Fun x X t) ad ->
+  ~ access m t ad.
+Proof. solve_inversion_not_access. Qed.
+
+Local Lemma inversion_not_access_call : forall m t1 t2 ad,
+  ~ access m (TM_Call t1 t2) ad ->
+  ~ access m t1 ad /\ ~ access m t2 ad.
+Proof. solve_inversion_not_access. Qed.
+
+Local Lemma inversion_not_access_seq : forall m t1 t2 ad,
   ~ access m (TM_Seq t1 t2) ad ->
   ~ access m t1 ad /\ ~ access m t2 ad.
-Proof.
-  intros * ?. split; intros F; inversion F; subst; eauto using access.
-Qed.
+Proof. solve_inversion_not_access. Qed.
 
 Ltac inversion_not_access :=
   match goal with
-    | H : _ |- ~ access _ TM_Nil _   =>
+    | H : _ |- ~ access _ TM_Unit _   =>
         intros F; inversion F 
     | H : _ |- ~ access _ (TM_Num _) _   =>
         intros F; inversion F 
@@ -112,39 +178,45 @@ Ltac inversion_not_access :=
         eapply inversion_not_access_new in H
     | H : ~ access _ (TM_Load _) _  |- _ =>
         eapply inversion_not_access_load in H
+    | H : _ |- ~ access _ (TM_Id _) _   =>
+        intros F; inversion F 
+    | H : ~ access _ (TM_Fun _ _ _) _ |- _ =>
+        eapply inversion_not_access_fun in H
+    | H : ~ access _ (TM_Call _ _) _ |- _ =>
+        eapply inversion_not_access_call in H as [? ?]
     | H : ~ access _ (TM_Asg _ _) _ |- _ =>
         eapply inversion_not_access_asg in H as [? ?]
     | H : ~ access _ (TM_Seq _ _) _ |- _ =>
         eapply inversion_not_access_seq in H as [? ?]
   end.
 
-Lemma not_access_new : forall m t ad,
+(* -------------------------------------------------------------------------- *)
+(* subst -------------------------------------------------------------------- *)
+(* -------------------------------------------------------------------------- *)
+
+Lemma access_subst : forall m x X t t' ad,
+  access m ([x := t'] t) ad ->
+  access m (TM_Call (TM_Fun x X t) t') ad.
+Proof.
+  intros. induction t; eauto using access; simpl in *;
+  try (destruct String.eqb; eauto using access);
+  try solve [ 
+    inversion_access; auto_specialize;
+    inversion_access; try inversion_access; eauto using access
+  ].
+Qed.
+
+Lemma not_access_subst : forall m id t x ad,
   ~ access m t ad ->
-  ~ access m (TM_New t) ad.
+  ~ access m x ad ->
+  ~ access m ([id := x] t) ad.
 Proof.
-  intros * ? ?. inversion_access. eauto.
+  intros. induction t; trivial;
+  try solve [
+    inversion_not_access;
+    eauto using not_access_new, not_access_load, not_access_asg,
+      not_access_call, not_access_seq
+  ];
+  simpl; destruct String.eqb; trivial.
+  inversion_not_access. eauto using not_access_fun.
 Qed.
-
-Lemma not_access_load : forall m t ad,
-  ~ access m t ad ->
-  ~ access m (TM_Load t) ad.
-Proof.
-  intros * ? ?. inversion_access. eauto.
-Qed.
-
-Lemma not_access_asg : forall m l r ad,
-  ~ access m l ad ->
-  ~ access m r ad ->
-  ~ access m (TM_Asg l r) ad.
-Proof.
-  intros * ? ? ?. inversion_access; eauto.
-Qed.
-
-Lemma not_access_seq : forall m t1 t2 ad,
-  ~ access m t1 ad ->
-  ~ access m t2 ad ->
-  ~ access m (TM_Seq t1 t2) ad.
-Proof.
-  intros * ? ? ?. inversion_access; eauto.
-Qed.
-
