Disjoint.v
@@ -3,7 +3,7 @@ From Coq Require Import Lia.
 
 From Elo Require Import Array.
 From Elo Require Import Map.
-From Elo Require Import Core0.
+From Elo Require Import Core.
 From Elo Require Import Access.
 From Elo Require Import Compat.
 From Elo Require Import WBA.
@@ -23,11 +23,11 @@ Local Lemma none_disjoint_memory_preservation : forall m m' ths t' tid,
 Proof.
   intros * ? ? Hmstep tid1 tid2 ? ? ?. inversion Hmstep; subst.
   destruct (Nat.eq_dec tid tid1), (Nat.eq_dec tid tid2); subst; eauto.
-  - rewrite (get_set_neq TM_Nil); rewrite (get_set_eq TM_Nil) in *;
+  - rewrite (get_set_neq TM_Unit); rewrite (get_set_eq TM_Unit) in *;
     eauto using mstep_none_inherits_access.
-  - rewrite (get_set_eq TM_Nil); rewrite (get_set_neq TM_Nil) in *;
+  - rewrite (get_set_eq TM_Unit); rewrite (get_set_neq TM_Unit) in *;
     eauto using mstep_none_preserves_not_access.
-  - rewrite (get_set_neq TM_Nil) in *; eauto.
+  - rewrite (get_set_neq TM_Unit) in *; eauto.
 Qed.
 
 Local Lemma load_disjoint_memory_preservation : forall m m' ths t' tid ad v,
@@ -38,11 +38,11 @@ Local Lemma load_disjoint_memory_preservation : forall m m' ths t' tid ad v,
 Proof.
   intros * ? ? Hmstep tid1 tid2 ? ? ?. inversion Hmstep; subst.
   destruct (Nat.eq_dec tid tid1), (Nat.eq_dec tid tid2); subst; eauto.
-  - rewrite (get_set_neq TM_Nil); rewrite (get_set_eq TM_Nil) in *;
+  - rewrite (get_set_neq TM_Unit); rewrite (get_set_eq TM_Unit) in *;
     eauto using mstep_load_inherits_access.
-  - rewrite (get_set_eq TM_Nil); rewrite (get_set_neq TM_Nil) in *;
+  - rewrite (get_set_eq TM_Unit); rewrite (get_set_neq TM_Unit) in *;
     eauto using mstep_load_preserves_not_access.
-  - rewrite (get_set_neq TM_Nil) in *; eauto.
+  - rewrite (get_set_neq TM_Unit) in *; eauto.
 Qed.
 
 Local Lemma alloc_disjoint_memory_preservation : forall m m' ths t' tid ad v,
@@ -53,18 +53,18 @@ Local Lemma alloc_disjoint_memory_preservation : forall m m' ths t' tid ad v,
   disjoint_memory m' (set ths tid t').
 Proof.
   intros * Hwba Hdis ? Hmstep tid1 tid2 ad' ? ?. inversion Hmstep; subst.
-  assert (~ access m (get TM_Nil ths tid1) (length m)).
+  assert (~ access m (get TM_Unit ths tid1) (length m)).
   { intros F. specialize (Hwba tid1 (length m) F). lia. }
-  assert (~ access m (get TM_Nil ths tid2) (length m)).
+  assert (~ access m (get TM_Unit ths tid2) (length m)).
   { intros F. specialize (Hwba tid2 (length m) F). lia. }
   destruct (Nat.eq_dec tid tid1), (Nat.eq_dec tid tid2); subst; eauto.
-  - rewrite (get_set_neq TM_Nil); rewrite (get_set_eq TM_Nil) in *; eauto.
+  - rewrite (get_set_neq TM_Unit); rewrite (get_set_eq TM_Unit) in *; eauto.
     destruct (Nat.eq_dec ad' (length m)); subst;
     eauto using inaccessible_address_add_2, mstep_alloc_inherits_access.
-  - rewrite (get_set_eq TM_Nil); rewrite (get_set_neq TM_Nil) in *; eauto.
+  - rewrite (get_set_eq TM_Unit); rewrite (get_set_neq TM_Unit) in *; eauto.
     destruct (Nat.eq_dec ad' (length m)); subst; eauto;
     eauto using inaccessible_address_add_1, mstep_alloc_preserves_not_access.
-  - rewrite (get_set_neq TM_Nil) in *; eauto.
+  - rewrite (get_set_neq TM_Unit) in *; eauto.
     eauto using inaccessible_address_add_1, inaccessible_address_add_2.
 Qed.
 
@@ -76,15 +76,15 @@ Local Lemma store_disjoint_memory_preservation : forall m m' ths t' tid ad v,
 Proof.
   intros * ? ? Hmstep tid1 tid2 ? ? ?. inversion Hmstep; subst.
   destruct (Nat.eq_dec tid tid1), (Nat.eq_dec tid tid2); subst; eauto.
-  - rewrite (get_set_neq TM_Nil); rewrite (get_set_eq TM_Nil) in *;
+  - rewrite (get_set_neq TM_Unit); rewrite (get_set_eq TM_Unit) in *;
     eauto 6 using mstep_store_address_access,
                   mstep_store_inherits_access,
                   inaccessible_address_set_2.
-  - rewrite (get_set_eq TM_Nil); rewrite (get_set_neq TM_Nil) in *;
+  - rewrite (get_set_eq TM_Unit); rewrite (get_set_neq TM_Unit) in *;
     eauto 6 using mstep_store_address_access,
                   mstep_store_preserves_not_access,
                   inaccessible_address_set_1.
-  - rewrite (get_set_neq TM_Nil) in *;
+  - rewrite (get_set_neq TM_Unit) in *;
     eauto 8 using mstep_store_address_access,
                   inaccessible_address_set_1,
                   inaccessible_address_set_2.
@@ -116,34 +116,34 @@ Proof.
   eauto using disjoint_memory_preservation'.
   intros tid1 tid2 ad Hacc Hneq.
   decompose sum (lt_eq_lt_dec (length ths) tid2); subst.
-  - rewrite (get_add_gt TM_Nil);
+  - rewrite (get_add_gt TM_Unit);
     try solve [rewrite set_preserves_length; trivial].
     intros ?. inversion_access.
   - erewrite <- set_preserves_length.
-    rewrite (get_add_eq TM_Nil).
-    eauto using noloc_then_not_access, noloc_for_block.
-  - rewrite (get_add_lt TM_Nil);
+    rewrite (get_add_eq TM_Unit).
+    eauto using noloc_for_block, noloc_then_not_access.
+  - rewrite (get_add_lt TM_Unit);
     try solve [rewrite set_preserves_length; trivial].
     decompose sum (lt_eq_lt_dec (length ths) tid1); subst.
-    + rewrite (get_add_gt TM_Nil) in Hacc;
+    + rewrite (get_add_gt TM_Unit) in Hacc;
       try solve [rewrite set_preserves_length; trivial].
       inversion_access.
     + erewrite <- set_preserves_length in Hacc.
-      rewrite (get_add_eq TM_Nil) in Hacc.
+      rewrite (get_add_eq TM_Unit) in Hacc.
       assert (~ access m' block ad) by 
-        eauto using noloc_then_not_access, noloc_for_block.
+        eauto using noloc_for_block, noloc_then_not_access.
       eauto.
-    + rewrite (get_add_lt TM_Nil) in Hacc;
+    + rewrite (get_add_lt TM_Unit) in Hacc;
       try solve [rewrite set_preserves_length; trivial].
       destruct (Nat.eq_dec tid tid1), (Nat.eq_dec tid tid2); subst; eauto.
-      * rewrite (get_set_neq TM_Nil); try lia.
-        rewrite (get_set_eq TM_Nil) in *; trivial.
+      * rewrite (get_set_neq TM_Unit); try lia.
+        rewrite (get_set_eq TM_Unit) in *; trivial.
         eauto using step_spawn_inherits_access.
-      * rewrite (get_set_eq TM_Nil); trivial.
-        rewrite (get_set_neq TM_Nil) in *; trivial.
+      * rewrite (get_set_eq TM_Unit); trivial.
+        rewrite (get_set_neq TM_Unit) in *; trivial.
         eauto using step_spawn_preserves_not_access.
-      * rewrite (get_set_neq TM_Nil); try lia.
-        rewrite (get_set_neq TM_Nil) in *; try lia.
+      * rewrite (get_set_neq TM_Unit); try lia.
+        rewrite (get_set_neq TM_Unit) in *; try lia.
         eauto.
 Qed.
 
