Util.v
@@ -1,0 +1,33 @@
+(* Miscellaneous Utilities *)
+
+Ltac auto_specialize :=
+  match goal with
+  | P : ?x, H : ?x -> _ |- _ => specialize (H P)
+  end.
+
+(* Unused
+
+Definition memory_has_values (m : mem) :=
+  forall ad, value (getTM m ad).
+
+Theorem memory_has_values_preservation : forall m m' t t' eff,
+  memory_has_values m ->
+  m / t ==[eff]==> m' / t' ->
+  memory_has_values m'.
+Proof.
+  intros. inversion_mstep; trivial.
+  - remember (EF_Alloc _ _) as eff.
+    induction_step; inversion Heqeff; subst; eauto. intros ad.
+    decompose sum (lt_eq_lt_dec ad (length m)); subst.
+    + rewrite (get_add_lt TM_Unit); trivial.
+    + rewrite (get_add_eq TM_Unit); trivial.
+    + rewrite (get_add_gt TM_Unit); eauto using value.
+  - remember (EF_Store _ _) as eff.
+    induction_step; inversion Heqeff; subst; eauto. intros ad'.
+    decompose sum (lt_eq_lt_dec ad' ad); subst.
+    + rewrite (get_set_lt TM_Unit); trivial.
+    + rewrite (get_set_eq TM_Unit); trivial.
+    + rewrite (get_set_gt TM_Unit); trivial.
+Qed.
+
+*)
